29 May commit-1

EasyTeach/SymEnc.ec
@@ -3,6 +3,313 @@
 (* Symmetric Encryption *)
 
 (* definitions, including games for judging correctness and IND-CPA
+  (indistinguishability under chosen plaintext attack) security *)
+
+prover ["Z3"].  (* no SMT solvers *)
+
+require import AllCore Distr DBool FSet SmtMap.
+require import Cyclic_group_prime.
+require import Prime_field.
+import Dgf_q.
+
+type  text.
+const zero:text.
+
+op ( ++ ) : text -> text -> text.
+op dtext : text distr.
+
+axiom xor_commutative : forall(x : text, y : text), x ++ y = y ++  x.
+axiom xor_associative (x,y,z : text) : (x ++ y) ++ z = x ++ (y ++ z).
+axiom xor_with_0: forall(x : text), x ++ zero = x.
+axiom xor_with_itself: forall(x:text), x ++ x = zero.
+axiom dtext_lossless : weight dtext = 1%r.
+
+
+module type RO = {
+ (* initialization *)
+ proc * init() : unit
+
+ (* application to a text *)
+ proc f(x : group) : text
+}.
+
+(* random function implemention using true randomness *)
+
+module RO : RO = {
+ (* mp is a finite map associating texts with texts *)
+ var mp : (group, text) fmap
+
+ proc init() : unit = {
+   mp <- empty;  (* empty map *)
+ }
+
+ proc f(x : group) : text = {
+   var y : text;
+   if (! x \in mp) {   (* give x a random value in *)
+     y <$ dtext;  (* mp if not already in mp's domain *)
+     mp.[x] <- y;
+   }
+   return oget mp.[x];
+ }
+}.
+
+type pub = group.
+type priv = gf_q.
+type cipher = group * text.
+
+module type ENC (RO : RO) = {
+ (* Alice private key generation *)
+
+ proc key_gen() : pub * priv {}
+
+ (* encryption *)
+ proc enc(A:group, x : text) : cipher {RO.f}
+
+ (* decryption *)
+ proc dec(p: priv, c : cipher) : text {RO.f}
+}.
+
+op ciph_def : group*text.  (* default ciphertext *)
+
+module (Enc : ENC) (RO : RO) = {
+ proc key_gen(): pub * priv = {
+   var priv_k: gf_q;
+   priv_k <$ dgf_q;
+   return (g^priv_k, priv_k); (*x is Alice's  private key *)
+ }
+
+ proc enc(A: pub, plain_text : text) : cipher ={
+     var k : gf_q; var c_1 : group; var c_2 : text;
+     k <$ dgf_q; (* Ephemeral key *)
+     c_1 <- g^k;
+     c_2 <@ RO.f(A^k); c_2 <- c_2 ++ plain_text;
+     return (c_1, c_2); (* Here A is Alice public key A = g^priv_key , this returns c_1=g^k and c_2= RO.f(A^k)++message *)
+ }
+
+     (* decryption *)
+
+ proc dec(priv_key: priv, c : cipher) : text ={
+     var y : group; var c_1 : group; var c_2, c_3 : text;
+     (c_1, c_2) <- c;
+     y <- c_1^(priv_key);
+     c_3 <@ RO.f(y);
+     return(c_3 ++ c_2); (* As y =c_1^(priv_key) and c_1 = g^k; c_3 ++ c_2 will  RO.f(c_1^(priv_key)) ++ RO.f(A^k) ++ message *)
+ }
+}.
+(* module for checking correctness of encryption, parameterized
+  by encryption scheme
+
+  correctness means main returns true with probability 1, without any
+  assumptions about value of x *)
+
+module Cor (Enc : ENC) = {
+ module E = Enc(RO)
+
+ proc main(x : text) : bool = {
+   var c  : cipher; var priv_key : priv; var pub_key : pub; var y, c_2: text;
+   (pub_key, priv_key) <@ E.key_gen();
+   c <@ E.enc(pub_key, x);
+   y <@ E.dec(priv_key, c);
+   return (x = y);
+ }
+}.
+
+(* encryption adversary, parameterized by encryption oracle, EO
+
+  choose may only call EO.enc_pre; guess may only call EO.enc_post *)
+
+module type ADV (RO : RO) = {
+ (* choose a pair of plaintexts, x1/x2 *)
+ proc * choose(pub_key : pub) : text * text {RO.f}
+
+ (* given ciphertext c based on a random boolean b (the encryption
+    using EO.genc of x1 if b = true, the encryption of x2 if b =
+    false), try to guess b *)
+ proc guess(c : cipher) : bool {RO.f}
+}.
+
+(* IND-CPA security game, parameterized by an encryption scheme Enc
+  and adversary Adv
+
+  an encryption scheme is secure iff the probability of main
+  returning true (Adv winning the game) is close to 1/2, i.e., Adv
+  isn't doing much better than always guessing the ciphertext comes
+  from the first plaintext, or of making a random guess
+
+  formally, we want that the absolute value of the difference between
+  the probability that main returns true and 1/2 to be small; this
+  says that Adv can neither win nor lose with probability much
+  different than 1/2 (if it could reliably lose, the addition of
+  a negation would result in an adversary that could reliably win)
+
+  because Adv can use EO to encrypt the plaintexts it chooses,
+  the encryption procedure of a secure encryption scheme is
+  necessarily probabilistic
+
+  Adv may directly use Enc (which is stateless) as much as it wants
+  (and in any case could simulate it), but the security theorem must
+   say it can't read/write the global variables of EncO *)
+
+
+
+module IND_CPA (Enc : ENC, Adv : ADV) = {
+ module E = Enc(RO)  (* connect Enc to RO *)
+ module A = Adv(RO)  (* connect Adv to RO *)
+
+ proc main() : bool = {
+   var b, b' : bool; var x1, x2 : text; var c : cipher;
+   var priv_key : priv; var pub_key : pub;
+  RO.init();
+  (pub_key,priv_key) <@ E.key_gen();
+   (x1, x2) <@ A.choose(pub_key);    (* let A choose plaintexts x1/x2 *)
+   b <$ {0,1};                (* choose boolean b *)
+   c <@ E.enc(pub_key, b ? x1 : x2); (* encrypt x1 if b = true, x2 if b = false *)
+   b' <@ A.guess(c);          (* give ciphertext to A, which returns guess *)
+   return b = b';             (* see if A guessed correctly, winning game *)
+ }
+}.
+
+
+lemma exp_equal (g: group, x_1, x_2 : gf_q) : x_1 = x_2 => g^x_1 = g^x_2 .
+proof. 
+move => -> //.
+qed.
+
+
+axiom pow_pow (g: group, v,v_1 : gf_q) :  g^v^v_1 = g^(v * v_1).
+
+lemma pow_com (g: group, v,v_1 : gf_q) : g^v^v_1 = g^v_1^v.
+    proof.
+    have -> :  g^v^v_1 = g^(v*v_1).
+      apply pow_pow.
+    have -> : v*v_1 = v_1*v.
+      apply gf_q_mult_comm.
+      smt(pow_pow).
+  qed.
+
+lemma pow_com_2 (g: group, v,v_1 : gf_q) : g^(v*v_1) = g^(v_1*v).
+    have -> : g^(v*v_1) = g^v^v_1.
+    smt(pow_pow).
+    have -> : g^(v_1*v) = g^v_1^v.
+    smt(pow_pow).
+    apply pow_com.
+  qed.
+  
+    
+
+
+lemma correctness : phoare[Cor(Enc).main : true ==> res] = 1%r.
+   proof.
+     proc.
+     inline*.
+     seq 2: (pub_key = g ^ priv_key).
+     auto.
+     auto.    
+     progress.
+     apply lossless.
+     sp.    
+     seq 3: (plain_text = x /\ c_1 = g ^ k /\ x0 = g ^ (priv_key * k)).
+     auto.
+     auto.
+     progress.
+     apply lossless.
+     rewrite pow_pow pow_com_2.
+     trivial.   
+     if.
+     seq 1 : 
+       (plain_text = x /\ c_1 = g ^ k /\ x0 = g ^ (priv_key * k) /\
+        x0 \notin RO.mp).
+     auto.
+     auto; progress; apply dtext_lossless.
+     sp; wp.
+     rcondf 1.
+         auto; progress.
+       search dom _.[_<-_].
+       apply mem_set.
+         smt( pow_pow pow_com_2).
+         auto.
+         progress.
+      
+       search _.[_<-_].
+       rewrite pow_pow pow_com_2.
+       rewrite get_set_sameE.
+         smt( xor_associative xor_with_itself xor_with_0).
+       hoare.
+         auto.
+         progress.
+         sp;wp.
+         progress.
+         rcondf 1.
+         auto.
+         progress.
+         rewrite pow_pow pow_com_2 //. 
+         auto.
+         progress.
+         rewrite pow_pow pow_com_2. 
+       search _.[_].
+       search oget.
+         rewrite get_some.
+trivial.
+       
+         rewrite  xor_associative xor_with_itself xor_with_0.
+       search oget.
+       
+       
+apply getE.
+apply map_set.
+       apply get_set_sameE.
+       apply oget_omap_some.
+apply oget_omap_some.
+       
+
+       
+(*
+search "_.[_<-_]" "_.[_]".
+search dom. (* instead of (\in) *)
+*)
+admit.
+auto; progress.
+admit.
+hoare.
+auto.
+trivial.
+
+
+
+
+     if.
+     auto; progress. apply dtext_lossless.
+
+
+
+     seq 2: (RO.mp.[x0] = Some y1).
+     auto.
+     auto.
+     progress.
+     apply dtext_lossless.
+     apply get_set_sameE.
+     sp.
+     if.
+     seq 2: (RO.mp.[x1] = Some y2).
+     auto.
+     auto.
+     progress.
+     apply dtext_lossless.
+     apply get_set_sameE.
+     auto.
+     progress.
+
+
+
+
+   module Game_2 = {
+
+ module EO = EncO(Enc)
+ (pub_key, priv_key) <@ EO.init();(* SymEnc.ec *)
+
+(* Symmetric Encryption *)
+
+(* definitions, including games for judging correctness and IND-CPA
    (indistinguishability under chosen plaintext attack) security *)
 
 prover ["Z3"].  (* no SMT solvers *)
@@ -209,37 +516,78 @@ lemma correctness : phoare[Cor(Enc(TRF)).main : true ==> res] = 1%r.
     proof.
       proc.
       inline*.
-      seq 2: ((pub_key = g ^ priv_k) /\ (priv_key = priv_k)).
+      seq 2: (pub_key = g ^ priv_key).
       auto.
       auto.    
       progress.
       apply lossless.
-      sp.    
-      seq 2: (c_10 = g ^ k).
+      sp.
+      seq 2: (c_10 = g ^ k /\  A = pub_key /\ plain_text = x /\ pub_key = g ^ priv_key).
       auto.
       auto.
       progress.
       apply lossless.
       sp.
-      if.
-      seq 2: (TRF.mp.[x0] = Some y1).
+      rcondt 1.
       auto.
+      progress.
+    
+      seq 2: (x0 = A ^ k /\  c_10 = g ^ k /\ A = pub_key /\ plain_text = x /\ pub_key = g ^ priv_key  /\ x0 \notin TRF.mp /\ TRF.mp.[x0] = Some y1).
+(*      seq 9: (c_1 = g ^ k /\ TRF.mp.[x0] = Some y1 /\ x1 = c_1 ^ priv_key /\ c_2 = y1 ).*)
+      auto.
+      auto.
+      progress.
+      apply dtext_lossless.
+      trivial.
+    
+
+      apply get_set_sameE.
+    
+      seq 0: (x1 = c_1^priv_key).   
+      auto.
+      auto.
+      if.
+      auto.
+      progress.
+      apply dtext_lossless.
+         
+    
+      seq 4: ((TRF.mp.[x0] = Some y1)/\ (c_20 = oget TRF.mp.[x0] ++ plain_text) /\ x0 = A ^ k).
+      auto.
+      wp.
       auto.
       progress.
       apply dtext_lossless.
       apply get_set_sameE.
       sp.
+      progress.
       if.
-      seq 2: (TRF.mp.[x1] = Some y2).
+      seq 1: ((TRF.mp.[x1] = Some y2)/\(c_20 = oget TRF.mp.[x0] ++ plain_text ) /\ (c_21 = c_2) /\ (x1 = c_1^ priv_key)).
       auto.
       auto.
       progress.
       apply dtext_lossless.
+      apply get_some.
       apply get_set_sameE.
+      apply oget_some.
+    
       auto.
       progress.
-      
-    
+      apply get_some.
+      seq 2: (TRF.mp.[x0] = Some y1).
+      auto.
+      auto.    
+      progress.
+    apply oget_same.
+      wp.
+      auto.    
+      progress.
+      auto.
+      progress.
+      auto.    
+      if.
+      seq 2: (TRF.mp.[x1] = Some y2).
+
     
     
     module Game_2 = {
